implem of new checker

theories/check.v
@@ -2,6 +2,14 @@ From mathcomp Require Import all_ssreflect.
 From det Require Import lang.
 From det Require Import run.
 
+(* TODO:
+A valid state for substitutions is mandatory?
+Given the following program execution
+(main X) => (p X, q X) => p X succeeds setting X to func, then
+OK, (r X \/ s X) => backchain for q X gives two solutions
+Is it important that the substitution in the Or note, X is a function?
+*)
+
 Lemma tm2RC_kp {t1 k} : 
   tm2RC t1 = Some (RCallable_Kp k) -> t1 = Tm_Kp k.
 Proof.
@@ -22,8 +30,123 @@ Proof.
   - move=> h b k; case X: tm2RC => //.
 Qed.
 
+Fixpoint has_cut A :=
+  match A with
+  | CutS => true
+  | CallS _ _ => false
+  | Bot | Dead => true
+  | OK | Top => false
+  | And A B0 B => has_cut A || (has_cut B0 && has_cut B)
+  | Or _ _ _ => is_ko A
+  end.
+
+
+Lemma has_cut_cut {B}: has_cut (cutr B).
+Proof. 
+  elim: B => //=.
+  - move=> ?????; rewrite !is_ko_cutr//.
+  - by move=> A ->.
+Qed.
+
+Lemma has_cut_dead {A}: is_dead A -> has_cut A.
+Proof.
+  elim: A => //=.
+  - move=> A HA s B HB/andP[/is_dead_is_ko->/is_dead_is_ko->]//.
+  - move=> A HA B0 _ B HB dA; rewrite HA//.
+Qed.
+Lemma has_cut_cutl {A}: has_cut A -> has_cut (cutl A).
+Proof.
+  elim: A => //.
+    move=> A HA s B HB/=/andP[kA kB]; rewrite fun_if/= is_ko_cutr kA !is_ko_cutl// if_same//.
+  move=> A HA B0 HB0 B HB /=/orP[].
+    by move=>/HA->.
+  move=>/andP[cB0 cB].
+  rewrite HB0//HB//orbT//.
+Qed.
+
+Lemma expand_has_cut {u A s}: 
+  has_cut A -> has_cut (get_state (expand u s A)) \/ is_cutbrothers (expand u s A).
+Proof.
+  elim: A s; try by move=> /=; auto.
+  - move=> A HA s1 B HB s /=/andP[kA kB].
+    case: ifP => dA.
+      rewrite (is_ko_expand _ kB)/=kA kB; auto.
+    rewrite (is_ko_expand _ kA)/=kA kB; auto.
+  - move=> A HA B0 _ B HB s /=/orP[].
+      move=> /(HA s); case: expand => [s1|s1||s1] C/= []//; auto => cC.
+      - by rewrite cC /=; left.
+      - by rewrite cC /=; left.
+      left; rewrite get_state_And /=.
+      by case: ifP; rewrite ?cC // has_cut_cutl.
+    case/andP=> cB0 cB.
+    case: expand => [s1|s1||s1] C/=; rewrite ?cB ?cB0 ?orbT; auto.
+    move: (HB s1 cB).
+    by case: expand => [s2|s2||s2] D /=; auto => -[]// ->; rewrite cB0 orbT; left.
+Qed.
+
+Lemma has_cut_success {A}:
+  has_cut A -> success A = false.
+Proof.
+  elim: A => //.
+  - move=> A HA s B HB /=/andP[kA kB].
+    rewrite !is_ko_success// if_same//.
+  - move=> A HA B0 HB0 B HB /=/orP[].
+      by move=>/HA->.
+    by move=>/andP[] _/HB->; rewrite andbF.
+Qed.
+
+Lemma success_has_cut {A}:
+  success A -> has_cut A = false.
+Proof.
+  elim: A => //.
+  - move=> A HA s B HB/=; case: ifP => dA.
+      rewrite is_dead_is_ko//=; apply: success_is_ko.
+    move=>/success_is_ko->//.
+  - by move=> A HA B0 HB0 B HB/=/andP[]/HA->/HB->; rewrite andbF.
+Qed.
+
+Lemma has_cut_next_alt {s A s' B}: 
+  has_cut A -> next_alt s A = Some (s', B) -> has_cut B.
+Proof.
+  elim: A s B s' => //.
+  - move=>/=[]?//?? _ [_<-]//.
+  - move=> A HA s1 B HB s C s' /=.
+    move=>/andP[kA kB].
+    by rewrite !is_ko_next_alt//; rewrite !if_same//.
+  - move=> A HA B0 HB0 B HB s C s' /=.
+    case: ifP => //= dA /orP[].
+      move=> cA.
+      have:= HA s _ _ cA.
+      case: next_alt => // [[s2 D]|].
+        move=>/(_ _ _ erefl) cD.
+        case: ifP => //= fA.
+          case: ifP => //= fB0 [??]; subst.
+          by rewrite /= cD.
+        case: next_alt => //[[s3 E]|].
+          by move=>[??]; subst; rewrite/=cA.
+        by case: ifP => fB //=[??]; subst; rewrite /= cD.
+      move=> _; case: ifP => //= fA.
+      case: next_alt => //= [[s2 D]][??]; subst => /=.
+      by rewrite cA.
+    move=>/andP[cB0 cB].
+    case: ifP => /= fA.
+      by case: next_alt => //= [[s1 D]]; case: ifP => // fB0 [_ <-]/=; rewrite cB0 orbT.
+    have:= HB s _ _ cB.
+    case: next_alt => //= [[s1 D]|].
+      by move=> /(_ _ _ erefl) cD [_ <-]/=; rewrite cB0 cD orbT.
+    by move=> _; case: next_alt => // [[s1 D]]; case: ifP => // fB0 [_ <-]/=; rewrite cB0 orbT.
+Qed.
+
+
 Section checker.
   Definition sigV := V -> option S.
+
+  Fixpoint get_prop_rightmost sig := (*this is the signature of predicate that should end in prop...*)
+    match sig with
+    | b (d r) => r
+    | b Exp => Func (*TODO: type error*)
+    | arr _ _ s => get_prop_rightmost s
+    end.
 
   Fixpoint is_det_sig (sig:S) : bool :=
     match sig with
@@ -33,12 +156,185 @@ Section checker.
     | arr _ _ s => is_det_sig s
     end.
 
-  Fixpoint getS_Callable (sP: sigT) (t: Callable) : option S :=
-    match t with
-    | Callable_Kp pn => Some (sP pn)
-    | Callable_V vn => None (*TODO: use sV vn instead*)
-    | Callable_Comb hd _ => getS_Callable sP hd
+  Fixpoint getS_tm (sP : sigT) (sV : sigV) (tm: Tm) : option S :=
+    match tm with
+    | Tm_Kd _ => Some (b Exp)
+    | Tm_Kp k => Some (sP k)
+    | Tm_V v => sV v
+    | Tm_Comb h _ => getS_tm sP sV h
     end.
+
+  Definition getS_Callable (sP: sigT) sV (t: Callable) : option S :=
+    getS_tm sP sV (Callable2Tm t).
+
+  Definition callable_is_det (sP: sigT) sV (t : Callable) :=
+    odflt false (omap is_det_sig (getS_Callable sP sV t)).
+
+  Definition maxD (d1 d2 : D) :=
+    match d1, d2 with
+    | Pred, _ | _, Pred => Pred
+    | Func, Func => Func
+    end.
+
+  Definition minD (d1 d2 : D) :=
+    match d1, d2 with
+    | Func, _ | _, Func => Func
+    | Pred, Pred => Pred
+    end.
+
+  Fixpoint incl_aux f1 f2 s1 s2 :=
+    match s1, s2 with
+    | b Exp, b Exp => true
+    | b(d D1), b(d D2) => f1 D1 D2 == D1
+    | arr i l1 r1, arr i l2 r2 => incl_aux f2 f1 l1 l2 && incl_aux f1 f2 r1 r2
+    | arr o l1 r1, arr o l2 r2 => incl_aux f1 f2 l1 l2 && incl_aux f1 f2 r1 r2
+    | _, _ => false (*TODO: this is type error*)
+    end.
+
+  Fixpoint min_max f1 f2 s1 s2 :=
+    match s1, s2 with
+    | b Exp, b Exp => b Exp
+    | b(d D1), b(d D2) => b(d(f1 D1 D2))
+    | arr i l1 r1, arr i l2 r2 => arr i (min_max f2 f1 l1 r1) (min_max f1 f2 r1 r2)
+    | arr o l1 r1, arr o l2 r2 => arr o (min_max f1 f2 l1 r1) (min_max f1 f2 r1 r2)
+    | _, _ => b Exp (*TODO: this is type error*)
+    end.
+
+  Definition incl := incl_aux minD maxD.
+  Definition min := min_max minD maxD.
+  Definition max := min_max maxD minD.
+  
+  Fixpoint strong s :=
+    match s with
+    | b Exp => b Exp
+    | b(d _) => b(d Func)
+    | arr i l r => arr i (weak l) (strong r)
+    | arr o l r => arr o (strong l) (strong r)
+    end
+  with weak s :=
+    match s with
+    | b Exp => b Exp
+    | b(d _) => b(d Pred) 
+    | arr i l r => arr i (strong l) (weak r)
+    | arr o l r => arr o (weak l) (weak r)
+    end.
+
+  Section test.
+    Definition SMap := 
+      (arr i (arr i (b Exp) (arr o (b Exp) (b(d Func)))) (arr i (b Exp) (arr o (b Exp) (b(d Func))))).
+    Definition WMap := 
+      (arr i (arr i (b Exp) (arr o (b Exp) (b(d Func)))) (arr i (b Exp) (arr o (b Exp) (b(d Pred))))).
+    Goal incl SMap WMap && ~~(incl WMap SMap). Proof. move=>//. Qed.
+    Goal (weak SMap) == WMap. Proof. move=> //=. Qed.
+  End test.
+
+  Fixpoint check_tm (sP:sigT) (sV:sigV) (tm : Tm) : (S * bool) :=
+    match tm with
+    | Tm_Kd k => (b Exp, true)
+    | Tm_Kp k => (sP k, true) 
+    | Tm_V v => (odflt (b Exp) (sV v), true) (*TODO: what to return if v is not in sV ??*)
+    | Tm_Comb l r => 
+      let '(s1, b1) := check_tm sP sV l in
+      match s1 with
+      | arr i tl tr => 
+        let '(s2, b2) := check_tm sP sV r in
+        let r := b1 && b2 && incl s2 tl in
+        if r then (tr, true)
+        else (weak tr, false)
+      | arr o tl tr => if b1 then (check_tm sP sV l) else (weak tr, false)
+      | _ => (b Exp, false) (*TODO: this is a typechecking error...*)
+      end
+    end.
+
+  Fixpoint assume_tm (sP:sigT) (sV:sigV) (tm : Tm) (s : S): sigV :=
+    match tm with
+    | Tm_Kd _ | Tm_Kp _ => sV
+    | Tm_V v =>
+      let t' := sV v in
+      fun x => if x == v then Some (odflt s (omap (fun x => min x s) t')) else sV x
+    | Tm_Comb l r =>
+      match s with
+      | arr i tl tr =>
+        let sP' := assume_tm sP sV l tl in
+        assume_tm sP sP' r tr
+      | arr o tl tr => assume_tm sP sV l tl
+      | _ => sV (*TODO: this is type error...*)
+      end
+    end.
+
+  Fixpoint assume_call (sP:sigT) (sV:sigV) (c : Callable) (s : S): sigV :=
+    match c with
+    | Callable_Kp _ => sV
+    | Callable_V v => sV
+    | Callable_Comb l r =>
+      match s with
+      | arr i tl tr => assume_call sP sV l tl
+      | arr o tl tr => 
+        let sV' := assume_call sP sV l tl in
+        assume_tm sP sV' r tr
+      | _ => sV (*TODO: this is type error*)
+      end
+    end.
+
+  Fixpoint assume_hd (sP:sigT) (sV:sigV) (s : S) (tm:Tm) : sigV :=
+    match tm with
+    | Tm_Kd _ => sV
+    | Tm_Kp _ => sV
+    | Tm_V v => fun x => if x == v then Some s else sV x
+    | Tm_Comb l r => 
+      match s with
+      | arr i tl tr => assume_hd sP (assume_hd sP sV tl l) tr r
+      | arr o tl _ => (assume_hd sP sV tl l)
+      | _ => sV (*TODO: wrong type, should be unreachable*)
+      end
+    end.
+
+  Fixpoint check_hd (sP:sigT) (sV:sigV) (s : S) (tm:Tm) : bool :=
+    match tm with
+    | Tm_Kd _ => true
+    | Tm_Kp k => sP k == s
+    | Tm_V v => odflt false (omap (fun x => x == s) (sV v))
+    | Tm_Comb l r => 
+      match s with
+      | arr i tl _ => (check_hd sP sV tl l)
+      | arr o tl tr => 
+        let '(t, b1) := check_tm sP sV r in 
+        (t == s) && b1 && (check_hd sP sV tl l)
+      | _ => false (*TODO: wrong type, should be unreachable*)
+      end
+    end.
+
+  Definition check_callable sP sV (c: Callable) : (D * sigV) :=
+    let '(x, b1) := check_tm sP sV (Callable2Tm c) in (*TODO: we hope b1 to be Func or Pred*)
+      if b1 then 
+        if x is b(d x) then
+          if getS_Callable sP sV c is Some s then
+            let sV' := assume_call sP sV c s in
+            (maxD x (get_prop_rightmost s), sV')
+          else (Pred, sV)
+        else (Pred, sV) (*TODO: type error*) 
+      else (Pred, sV).
+
+  Definition check_atom sP sV (a: A) (s:D) : (D * sigV) :=
+    match a with
+    | ACut => (Func, sV)
+    | ACall t => check_callable sP sV t
+    end. 
+
+  Fixpoint check_atoms sP sV l s :=
+    match l with
+    | [::] => (s, sV)
+    | x :: xs => 
+      let '(s', sV') := check_atom sP sV x s in
+      check_atoms sP sV' xs s'
+    end.
+
+  (* all bodies should have a cut followed by checked atoms *)
+  (* ACCEPTED: a1 ... an, !, b1 ... bm *)
+  (* we want that b1 ... bm is func *)
+  (* NOTE: flags about determinacy can be obtained from a1...an *)
+  Definition check_atoms_w_cut (sP :sigT) sV (l: seq A) :=
+    ((check_atoms sP sV l Func).1 == Func) && (ACut \in l).
 
   Fixpoint rcallable_is_det (sP: sigT) (t:RCallable) : bool :=
     match t with
@@ -46,233 +342,217 @@ Section checker.
     | RCallable_Kp k => is_det_sig (sP k)
     end.
 
-  Definition tm_is_det (sP: sigT) (t : Callable) :=
-    odflt false (omap is_det_sig (getS_Callable sP t)).
+  Definition empty_ctx : sigV := fun x => None.
+  
+  (* The rules passes the check if it is 
+     implementating a relation predicate.
+     Otherwiser its atoms should pass the check
+  *)
+  Definition check_rule sP sV head prems :=
+    (rcallable_is_det sP head == false) ||
+    check_atoms_w_cut sP sV prems.
 
-  Definition check_atom sP (a: A) :=
-    match a with
-    | ACut => true
-    | ACall t => tm_is_det sP t
-    end. 
-
-  Fixpoint check_atoms (sP :sigT) (s: seq A) :=
-    match s with
-    | [::] => false
-    | ACut :: xs => all (check_atom sP) xs || check_atoms sP xs
-    | ACall _ :: xs => check_atoms sP xs
-    end.
-
-
-  Definition check_rule sP head prems :=
-    (rcallable_is_det sP head == false) || 
-      check_atoms sP prems.
-
-  Definition check_rules sP rules :=
-    all (fun x => check_rule sP x.(head) x.(premises)) rules.
+  Definition check_rules sP sV rules :=
+    all (fun x => check_rule sP sV x.(head) x.(premises)) rules.
 
   Definition check_program sP := 
-    forall pr, check_rules sP (rules pr).
+    forall pr, check_rules sP empty_ctx (rules pr).
 End checker.
 
-Section check.
+(* a free alternative can be reached without encountering a cutr following SLD 
 
-  Fixpoint has_cut A :=
-    match A with
-    | CutS => true
-    | CallS _ _ => false
-    | Bot | Dead => true
-    | OK | Top => false
-    | And A B0 B => has_cut A || (has_cut B0 && has_cut B)
-    | Or _ _ _ => is_ko A
-    end.
+  "((A, !, A') ; B) , C" is OK since B is not free
+  "((A, A') ; B) , !, C" is OK because any alt from first conjunct dies
+  "((A, A') ; B) , C" is OK if B is dead already (cutr by predecessor of A for example)
+
+*)
+Fixpoint det_tree_aux (sP:sigT) (sV : sigV) A dd : D * sigV :=
+  match A with
+  | CutS => (Func, sV)
+  | CallS _ a => check_atom sP sV (ACall a) dd
+  | Top | Bot | OK => (dd, sV)
+  | Dead => (dd, sV)
+  | And A B0 B =>
+    if is_ko A then (dd, sV)
+    else
+      let '(dd', sV') := det_tree_aux sP sV A dd in
+      let '(ddB0, sVB0) := det_tree_aux sP sV' B0 dd' in
+      let '(ddB, sVB) := det_tree_aux sP sV' B dd' in
+      (maxD ddB0 ddB, sV')
+  | Or A _ B =>
+      let '(sVA, sV') := det_tree_aux sP sV A dd in
+      let '(sVB, _) := det_tree_aux sP sV B dd in
+      if has_cut A then (maxD sVA sVB, sV) else 
+      if (is_ko B) then (sVA, sV')
+      else (Pred, sV)
+  end.
+
+Definition det_tree sP A := (det_tree_aux sP empty_ctx A Func).1 == Func.
+
+Lemma no_alt_ko {sP A}: is_ko A -> det_tree sP A.
+Proof.
+  rewrite/det_tree.
+  elim: A => //.
+  + move=> A HA s B HB /=/andP[kA kB].
+    case X: det_tree_aux HA => //=[dA sVA]/(_ kA)/eqP?; subst.
+    case Y: det_tree_aux HB => //=[dB sVB]/(_ kB)/eqP?; subst.
+    rewrite kB; case: ifP => //.
+  + move=> A HA B0 HB0 B HB /= ->//.
+Qed.
+
+  Lemma no_alt_cut {sP A}: det_tree sP (cutr A).
+Proof. apply: no_alt_ko is_ko_cutr. Qed.
 
 
-  Lemma has_cut_cut {B}: has_cut (cutr B).
-  Proof. 
-    elim: B => //=.
-    - move=> ?????; rewrite !is_ko_cutr//.
-    - by move=> A ->.
-  Qed.
+Lemma no_alt_dead {sP A}: is_dead A -> det_tree sP A.
+Proof. move=>/is_dead_is_ko. apply: no_alt_ko. Qed.
 
-  Lemma has_cut_dead {A}: is_dead A -> has_cut A.
-  Proof.
-    elim: A => //=.
-    - move=> A HA s B HB/andP[/is_dead_is_ko->/is_dead_is_ko->]//.
-    - move=> A HA B0 _ B HB dA; rewrite HA//.
-  Qed.
+Lemma all_det_nfa_big_and {sP sV l r} p: 
+  (check_atoms sP sV l r).1 = Func -> 
+    (det_tree_aux sP sV (big_and p l) r).1 = (Func).
+Proof.
+  elim: l sV r => //=.
+  move=> A As IH sV r.
+  case X: check_atom => [dA sVA].
+  move=> {}/IH H.
+  case: A X => //=.
+    move=> [??]; subst => /=.
+    case: det_tree_aux H => //=-[]//.
+  move=> c.
+  rewrite/check_callable.
+  case Z: check_tm => [S []]/=; last first.
+    move=> [??]; subst.
+    case: det_tree_aux H => -[]//.
+  case: S Z => //=; last first.
+    move=> m s1 s2 Z [??]; subst.
+    case: det_tree_aux H => -[]//.
+  move=> []//=.
+    move=> +[??]; subst.
+    case: det_tree_aux H => -[]//.
+  move=> d.
+  case X: getS_Callable => //=[SS|].
+    move=> +[??]; subst.
+    case: det_tree_aux H => //=-[]//.
+  move=> +[??]; subst.
+  case: det_tree_aux H => //=-[]//.
+Qed.
 
-  (* a free alternative can be reached without encountering a cutr following SLD 
+Lemma cut_followed_by_det_has_cut {sP sV l} p:
+  check_atoms_w_cut sP sV l -> has_cut (big_and p l).
+Proof. move=>/andP[] _; elim: l => //=-[]//= x xs IH /IH->//. Qed.
+
+Lemma cut_followed_by_det_nfa_and {sP sV bo} p:
+  check_atoms_w_cut sP sV bo -> (det_tree_aux sP sV (big_and p bo) Func).1 = Func.
+Proof. move=>/andP[]/eqP/all_det_nfa_big_and//. Qed.
+
+Lemma tiki_taka {modes sP sV u s t q hd s2}:
+  tm2RC (deref s (Callable2Tm t)) = Some q ->
+  H u (modes q) q hd s = Some s2 ->
+  getS_Callable sP sV t = Some (b (d Func)) -> rcallable_is_det sP hd.
+Proof.
+  generalize (modes q) => {}modes/=.
+  elim: modes q hd t s s2 => //=.
+    move=> []//=k []//= k1 t s1 s2; case: eqP => //=<-.
+    move=>/deref_kp [].
+      case: t => //= k2[->] _ [->]//.
+    move=> [v[]]; case: t => //= v1 [->] H _.
+    rewrite /getS_Callable/=.
+    admit.
+  move=> []//ml IH []//h1 b1 []//=h2 b2 t s1 s2 H1 H2 H3.
+    move: H2; case e: H => //=[s1']H2.
+    case: t H1 H3 => //=.
+      admit.
+    move=> c t.
+    case H : tm2RC => //=[h1'] [??]; subst => /=H1.
+    apply: IH H e H1.
+  move: H2; case e: H => //=[s1']H2.
+  case: t H1 H3 => //=.
+    admit.
+  move=> c t.
+  case H : tm2RC => //=[h1'] [??]; subst => /=H1.
+  apply: IH H e H1.
+Admitted.
+
+(* TODO: HERE
+  Given a deterministic predicate p,
+  Let t, be a valid call to p,
+  Given a list of valid rules in a program p, then
+  backchaining produces a deterministic tree!
+*)
+Lemma is_det_det_tree {u sP t s1 sV} {p:program}:
+  (* TODO: s1 and sV should be linked somehow *)
+  check_rules sP sV p.(rules) -> (check_callable sP sV t).1 = Func -> 
+    (det_tree_aux sP sV (big_or u p s1 t) Func).1 = Func.
+Proof.
+  rewrite/check_callable.
+  rewrite /big_or/F.
+  case X: tm2RC => //[rc].
+  case: p => rules modes sig1 /=.
+  generalize {| rules := rules; modes := modes; sig := sig1 |} as pr => pr.
+  clear -X.
+  elim: rules modes s1 t pr rc X => //=.
+  move=> [] hd bo rules IH modes s/= t p q X /andP[H1 H1'] H2.
+  case H: H => /= [s2|]; last first.
+    apply: IH X H1' H2.
+  clear IH.
+  move: H.
+  (* set t' := deref s t. *)
+  move: H1 => /orP[]; last first.
+    move=> + _.
+    elim: rules sV H1' H2 bo => //=.
+      move=> sV _ _ bo.
+      move=>/(cut_followed_by_det_nfa_and p).
+      case: det_tree_aux => //=-[]//.
+    move=> [] hd1 bo1/= l IH sV /andP [H3 H4] H2 bo H1.
+    case H: H => [s3|]//=; last first.
+      by apply: IH.
+    rewrite (cut_followed_by_det_has_cut _ H1).
+    have:= cut_followed_by_det_nfa_and p H1.
+    case Y: det_tree_aux => //=[? sV']?; subst.
+    case Z: det_tree_aux => [d sV''].
+    move: H2; case W: check_tm => //=[d1 []]//.
+    case: d1 W => //=-[]// d1.
+    case: d Z => //.
+    suffices Hz : (getS_Callable sP sV t = Some (b (lang.d d1))).
+      rewrite Hz/=.
+      case: d1 Hz => //= Hz Z H5 _.
+      move: H3 => /orP[]H3; last first.
+        have:= IH sV.
+        rewrite H4 H5/= Hz/= => /(_ isT erefl _ H3).
+        rewrite Z//.
+      admit.
+    admit.
+  move=> /eqP H3 H4.
+  case W: det_tree_aux => [[|]sV1]//.
+  move: H2; case C: check_tm => [S []]//.
+  case: S C => //=-[]//=d C.
+  case Z: getS_Callable => //=[S].
+  case: d C => //= C.
+  case K: get_prop_rightmost => //=.
   
-    "((A, !, A') ; B) , C" is OK since B is not free
-    "((A, A') ; B) , !, C" is OK because any alt from first conjunct dies
-    "((A, A') ; B) , C" is OK if B is dead already (cutr by predecessor of A for example)
-  
+  case: S Z => //=.
+  have:= tiki_taka X H4 .
+  have /= := tiki_taka X H2 H4; congruence.
+
+  case r: rules => //=.
+
+  elim: t sV => //=.
+  - move=> k sV.
+Qed.
+
+  (* 
+    Given a checked program, and a deterministic tree,
+    then calling expand produces a tree which is still deterministic.
   *)
-  Fixpoint no_free_alt (sP:sigT) A :=
-    match A with
-    | CutS => true
-    | CallS _ a => tm_is_det sP a
-    | Top | Bot | OK => true
-    | Dead => true
-    | And A B0 B =>
-      (is_ko A) || 
-        [&& (has_cut B0 && has_cut B) || no_free_alt sP A, 
-          no_free_alt sP B & no_free_alt sP B0]
-    | Or A _ B =>
-        no_free_alt sP A && 
-          if has_cut A then no_free_alt sP B else (B == cutr B) (* TODO: should be is_ko *)
-    end.
-
-  Lemma no_alt_cut {sP A}: no_free_alt sP (cutr A).
-  Proof.
-    elim: A => //.
-    + by move=> A HA s B HB /=; rewrite HA HB cutr2 eqxx if_same.
-    + move=> A HA B0 HB0 B HB /=; rewrite is_ko_cutr//.
-  Qed.
-
-  Lemma no_alt_dead {sP A}: is_dead A -> no_free_alt sP A.
-  Proof.
-    elim: A => //.
-    + move=> A HA s B HB /=/andP[dA]; rewrite HA// has_cut_dead//.
-    + move=> A HA B0 HB0 B HB /=dA; rewrite is_dead_is_ko//.
-  Qed.
-
-  Lemma has_cut_cutl {A}: has_cut A -> has_cut (cutl A).
-  Proof.
-    elim: A => //.
-      move=> A HA s B HB/=/andP[kA kB]; rewrite fun_if/= is_ko_cutr kA !is_ko_cutl// if_same//.
-    move=> A HA B0 HB0 B HB /=/orP[].
-      by move=>/HA->.
-    move=>/andP[cB0 cB].
-    rewrite HB0//HB//orbT//.
-  Qed.
-
-  Lemma all_det_nfa_big_and {p sP l}: all (check_atom sP) l -> no_free_alt sP (big_and p l).
-  Proof.
-    elim: l => //= a l IH/andP[] H1 H2.
-    case: a IH H1 => //= [|t] IH H1; rewrite ?H1 IH//=orbT//.
-  Qed.
-
-  Lemma cut_followed_by_det_has_cut {sP p l}:
-      check_atoms sP l -> has_cut (big_and p l).
-  Proof. by elim: l => //= -[]//= _ l H/H->. Qed.
-
-  Lemma cut_followed_by_det_nfa_and {sP p bo} :
-    check_atoms sP bo -> no_free_alt sP (big_and p bo).
-  Proof.
-    elim: bo => //=.
-    move=> [|t] /= l IH.
-      by move=>/orP[/all_det_nfa_big_and|/IH]->; rewrite orbT.
-    by move=> H; rewrite IH//!andbT andbb (cut_followed_by_det_has_cut H).
-  Qed.
-
-  Lemma no_free_alt_cutl {sP A}: no_free_alt sP (cutl A).
-  Proof.
-    elim: A => //.
-      move=> A HA s B HB/=.
-      rewrite fun_if/=HA HB cutr2 eqxx no_alt_cut if_same.
-      case: ifP => //dA.
-      rewrite has_cut_dead//no_alt_dead//.
-    move=> A HA B0 HB0 B HB /=.
-    rewrite HA HB HB0 !orbT//.
-  Qed.
-
-  Variable u : Unif.
-
-  Lemma tiki_taka {sP s s3 modes t q hd1}:
-    let t' := tm2RC (deref s (Callable2Tm t)) in
-    t' = Some q ->
-    tm_is_det sP t ->
-      H u modes q hd1 s = Some s3 ->
-        rcallable_is_det sP hd1.
-  Proof.
-    move=>/=.
-    elim: modes q hd1 t s s3 => //=.
-      move=> []//=k []//= k1 t s1 s2; case: eqP => //=<-.
-      move=>/deref_kp [].
-        case: t => //= k2 [->]//.
-      move=> [v[]]; case: t => //.
-    move=> []//ml IH []//h1 b1 []//=h2 b2 t s1 s2 H1 H2 H3.
-      move: H3; case e: H => //=[s1'] H3.
-      case: t H1 H2 => //= c t.
-      case H : tm2RC => //=[h1'] [??]; subst => /=.
-      rewrite/tm_is_det/=.
-      case X: getS_Callable => //[S] H1.
-      apply: IH H _ e.
-      rewrite/tm_is_det X//.
-    move: H3; case e: H => //=[s1'] H3.
-    case: t H1 H2 => //= c t.
-    case H : tm2RC => //=[h1'] [??]; subst => /=.
-    rewrite/tm_is_det/=.
-    case X: getS_Callable => //[S] H1.
-    apply: IH H _ e.
-    rewrite/tm_is_det X//.
-  Qed.
-
-
-  Lemma is_det_no_free_alt {sP t s1} {p:program}:
-    check_rules sP p.(rules) -> tm_is_det sP t -> 
-      no_free_alt sP (big_or u p s1 t).
-  Proof.
-    rewrite /big_or/F.
-    case X: tm2RC => //=[q].
-    case: p => rules modes sig1 /=.
-    generalize {| rules := rules; modes := modes; sig := sig1 |} as pr => pr.
-    clear -X.
-    elim: rules modes s1 t pr q X => //=.
-    move=> [] hd bo rules IH modes s/= t p q X /andP[H1 H1'] H2.
-    case H: H => /= [s2|]; last first.
-      apply: IH X H1' H2.
-    clear IH.
-    move: H.
-    (* set t' := deref s t. *)
-    move: H1 => /orP[]; last first.
-      move=> + _.
-      elim: rules H1' bo => //=.
-        move=> _ bo.
-        apply cut_followed_by_det_nfa_and.
-      move=> [] hd1 bo1/= l IH /andP [H3 H4] bo H1.
-      case H: H => [s3|]//=; last first.
-        by apply: IH.
-      rewrite (cut_followed_by_det_has_cut H1).
-      rewrite cut_followed_by_det_nfa_and//=.
-      rewrite IH//=.
-      move: H3 => /orP[] => //.
-      move=> /eqP H3; exfalso.
-      have /= := tiki_taka X H2 H; congruence.
-    move=> /eqP H3 H4.
-    have /= := tiki_taka X H2 H4; congruence.
-  Qed.
-
-  Lemma expand_has_cut {A s}: 
-    has_cut A -> has_cut (get_state (expand u s A)) \/ is_cutbrothers (expand u s A).
-  Proof.
-    elim: A s; try by move=> /=; auto.
-    - move=> A HA s1 B HB s /=/andP[kA kB].
-      case: ifP => dA.
-        rewrite (is_ko_expand _ kB)/=kA kB; auto.
-      rewrite (is_ko_expand _ kA)/=kA kB; auto.
-    - move=> A HA B0 _ B HB s /=/orP[].
-        move=> /(HA s); case: expand => [s1|s1||s1] C/= []//; auto => cC.
-        - by rewrite cC /=; left.
-        - by rewrite cC /=; left.
-        left; rewrite get_state_And /=.
-        by case: ifP; rewrite ?cC // has_cut_cutl.
-      case/andP=> cB0 cB.
-      case: expand => [s1|s1||s1] C/=; rewrite ?cB ?cB0 ?orbT; auto.
-      move: (HB s1 cB).
-      by case: expand => [s2|s2||s2] D /=; auto => -[]// ->; rewrite cB0 orbT; left.
-  Qed.
-
-  Lemma expand_no_free_alt {sP s1 A r} : 
-    check_program sP -> no_free_alt sP A -> 
+  Lemma expand_det_tree {sP s1 A r} : 
+    check_program sP -> det_tree sP A -> 
       expand u s1 A = r ->
-        no_free_alt sP (get_state r).
+        det_tree sP (get_state r).
   Proof.
     move=> H + <-; clear r.
     elim: A s1 => //.
     - move=> p t s1 /=.
-      apply: is_det_no_free_alt.
+      apply: is_det_det_tree.
       by have:= H p.
     - move=> A HA s B HB s1 /=/andP[fA].
       case: ifP => //= cA.
@@ -298,40 +578,16 @@ Section check.
         rewrite /= (HB s1) //.
         have := @expand_has_cut _ s1 cB.
         case H1: (is_cutbrothers (expand u s1 B)).
-          move=>_/=; rewrite has_cut_cutl// no_free_alt_cutl no_free_alt_cutl !orbT//.
+          move=>_/=; rewrite has_cut_cutl// det_tree_cutl det_tree_cutl !orbT//.
         move=> []//H2; rewrite H2 fB0 cB0 orbT//.
       have:= HA s fA.
       case X: expand => //= [|||s1 C] H1; try rewrite H1 orbT fB fB0 orbT//.
       have:= HB s1 fB; case Y: expand => //= H2; try rewrite fB0 H2 H1 orbT !orbT//.
-      rewrite !no_free_alt_cutl H2 !orbT//.
-  Qed.
-
-  Goal forall sP s, no_free_alt sP (Or OK s OK) == false.
-  Proof. move=> ?? //=. Qed.
-
-  Lemma has_cut_success {A}:
-    has_cut A -> success A = false.
-  Proof.
-    elim: A => //.
-    - move=> A HA s B HB /=/andP[kA kB].
-      rewrite !is_ko_success// if_same//.
-    - move=> A HA B0 HB0 B HB /=/orP[].
-        by move=>/HA->.
-      by move=>/andP[] _/HB->; rewrite andbF.
-  Qed.
-
-  Lemma success_has_cut {A}:
-    success A -> has_cut A = false.
-  Proof.
-    elim: A => //.
-    - move=> A HA s B HB/=; case: ifP => dA.
-        rewrite is_dead_is_ko//=; apply: success_is_ko.
-      move=>/success_is_ko->//.
-    - by move=> A HA B0 HB0 B HB/=/andP[]/HA->/HB->; rewrite andbF.
+      rewrite !det_tree_cutl H2 !orbT//.
   Qed.
 
   Lemma expand_next_alt {sP s1 A s2 B} : 
-    check_program sP -> no_free_alt sP A ->
+    check_program sP -> det_tree sP A ->
       expand u s1 A = Success s2 B -> forall s3, next_alt s3 B = None.
   Proof.
     move=> H.
@@ -368,7 +624,7 @@ Section check.
 
   Lemma expandedb_next_alt_done {sP s A s1 B b}: 
     check_program sP -> 
-      no_free_alt sP A -> expandedb u s A (Done s1 B) b ->
+      det_tree sP A -> expandedb u s A (Done s1 B) b ->
         forall s0, next_alt s0 B = None.
   Proof.
     remember (Done _ _) as d eqn:Hd => Hz + H.
@@ -378,45 +634,14 @@ Section check.
       apply: expand_next_alt Hz fA HA.
     } 
     - move=> s1 s2 r A B b HA HB IH s3 C ? fA; subst.
-      apply: IH erefl (expand_no_free_alt Hz fA HA).
+      apply: IH erefl (expand_det_tree Hz fA HA).
     - move=> s1 s2 r A B b HA HB IH s3 C ? fA; subst.
-      apply: IH erefl (expand_no_free_alt Hz fA HA).
+      apply: IH erefl (expand_det_tree Hz fA HA).
   Qed.
 
-  Lemma has_cut_next_alt {s A s' B}: 
-    has_cut A -> next_alt s A = Some (s', B) -> has_cut B.
-  Proof.
-    elim: A s B s' => //.
-    - move=>/=[]?//?? _ [_<-]//.
-    - move=> A HA s1 B HB s C s' /=.
-      move=>/andP[kA kB].
-      by rewrite !is_ko_next_alt//; rewrite !if_same//.
-    - move=> A HA B0 HB0 B HB s C s' /=.
-      case: ifP => //= dA /orP[].
-        move=> cA.
-        have:= HA s _ _ cA.
-        case: next_alt => // [[s2 D]|].
-          move=>/(_ _ _ erefl) cD.
-          case: ifP => //= fA.
-            case: ifP => //= fB0 [??]; subst.
-            by rewrite /= cD.
-          case: next_alt => //[[s3 E]|].
-            by move=>[??]; subst; rewrite/=cA.
-          by case: ifP => fB //=[??]; subst; rewrite /= cD.
-        move=> _; case: ifP => //= fA.
-        case: next_alt => //= [[s2 D]][??]; subst => /=.
-        by rewrite cA.
-      move=>/andP[cB0 cB].
-      case: ifP => /= fA.
-        by case: next_alt => //= [[s1 D]]; case: ifP => // fB0 [_ <-]/=; rewrite cB0 orbT.
-      have:= HB s _ _ cB.
-      case: next_alt => //= [[s1 D]|].
-        by move=> /(_ _ _ erefl) cD [_ <-]/=; rewrite cB0 cD orbT.
-      by move=> _; case: next_alt => // [[s1 D]]; case: ifP => // fB0 [_ <-]/=; rewrite cB0 orbT.
-  Qed.
 
-  Lemma no_free_alt_next_alt {sP s1 A s2 B}:
-    no_free_alt sP A -> next_alt s1 A = Some (s2, B) -> no_free_alt sP B.
+  Lemma det_tree_next_alt {sP s1 A s2 B}:
+    det_tree sP A -> next_alt s1 A = Some (s2, B) -> det_tree sP B.
   Proof.
     elim: A s1 B s2 => //.
     - move=> []//??? _ [_<-]//.
@@ -476,11 +701,10 @@ Section check.
       by rewrite fD orbT fB0 orbT.
   Qed.
 
-
   Lemma expand_next_alt_failed {sP A B C s s'}:
     check_program sP ->
-      no_free_alt sP A -> expand u s A = Failure B ->
-        forall sN, next_alt sN B = Some (s', C) -> no_free_alt sP C.
+      det_tree sP A -> expand u s A = Failure B ->
+        forall sN, next_alt sN B = Some (s', C) -> det_tree sP C.
   Proof.
     move=> Hz.
     elim: A B C s s' => //.
@@ -508,7 +732,7 @@ Section check.
         case: ifP => // dB.
         have dDe := @is_dead_dead E.
           case nB : next_alt => //= [[s2 F]] [_<-]/=.
-          rewrite no_alt_dead// has_cut_dead// (no_free_alt_next_alt fB nB)//.
+          rewrite no_alt_dead// has_cut_dead// (det_tree_next_alt fB nB)//.
       move=> cA /eqP->.
       have:= HA _ _ s _ fA _ sN.
       case X: expand => // [E] /(_ _ _ _ erefl) + [<-]/=.
@@ -530,7 +754,7 @@ Section check.
             case nE: next_alt => [[s3 F]|]//.
             by case: ifP => //FB0 [_<-]/=; rewrite cB0 fB0 orbT.
           case Y: next_alt => //[[s3 F]|].
-            by move=>[_ <-]/=; rewrite cB0 (has_cut_next_alt cB Y) fB0 (no_free_alt_next_alt fB Y) orbT.
+            by move=>[_ <-]/=; rewrite cB0 (has_cut_next_alt cB Y) fB0 (det_tree_next_alt fB Y) orbT.
           by case: next_alt => // [[s3 F]]; case:ifP=>//_[_<-]/=; rewrite cB0 fB0 orbT.
         have:= HB _ _ s1 _ fB _ sN.
         case Z: expand => // [F] /(_ _ _ _ erefl) + [<-]/=.
@@ -553,37 +777,37 @@ Section check.
           case: next_alt => //[[s4 G]] /(_ _ _ erefl) fG.
           by case: ifP => // _[_<-]/=; rewrite fB0 fG orbT orbT.
         case Y: (next_alt sN B) => //[[s4 G]|].
-          by move=> _ [_<-]/=; rewrite (no_free_alt_next_alt fB Y) fB0 (expand_no_free_alt Hz fA X) orbT orbT.
+          by move=> _ [_<-]/=; rewrite (det_tree_next_alt fB Y) fB0 (expand_det_tree Hz fA X) orbT orbT.
         case: next_alt => //[[s3 G]] /(_ _ _ erefl)fG; case:ifP=>//_[_<-]/=.
         by rewrite fG fB0 orbT orbT.
       move=> _.
       have:= HB _ _ s1 _ fB _ sN.
       case Z: expand => // [F] /(_ _ _ _ erefl) {}HB [<-]/=.
-      have /= fE := expand_no_free_alt Hz fA X.
+      have /= fE := expand_det_tree Hz fA X.
       case: ifP => //dE; case:ifP=>FE.
         case W: next_alt => //[[s3 G]]; case:ifP=>//_[_<-]/=.
-        by rewrite fB0 (no_free_alt_next_alt fE W) orbT orbT.
+        by rewrite fB0 (det_tree_next_alt fE W) orbT orbT.
       move: HB.
       case W: next_alt => //[[s3 G]|].
         move=> /(_ _ _ erefl) fG [_<-]/=; rewrite fG fB0 fE orbT orbT//.
       case T: next_alt => //[[s3 G]] => _; case:ifP => //[fB01][_<-]/=.
-      by rewrite fB0 (no_free_alt_next_alt fE T) orbT orbT.
+      by rewrite fB0 (det_tree_next_alt fE T) orbT orbT.
     Qed.
 
   Lemma expandedb_next_alt_failed {sP s A B C s' b1}: 
     check_program sP ->
-      no_free_alt sP A ->
+      det_tree sP A ->
         expandedb u s A (Failed B) b1 -> 
-          forall sN, next_alt sN B = Some (s', C) -> no_free_alt sP C.
+          forall sN, next_alt sN B = Some (s', C) -> det_tree sP C.
   Proof.
     remember (Failed _) as f eqn:Hf => Hz + H.
     elim: H B C s' Hf => //; clear -Hz.
     - move=> s A B HA ? C s' [<-] fA nB.
       apply: expand_next_alt_failed Hz fA HA nB.
     - move=> s s' r A B b HA HB IH C D s1 ? fA sN nB; subst.
-      apply: IH erefl (expand_no_free_alt Hz fA HA) _ nB.
+      apply: IH erefl (expand_det_tree Hz fA HA) _ nB.
     - move=> s s' r A B b HA HB IH C D s1 ? fA sN nB; subst.
-      apply: IH erefl (expand_no_free_alt Hz fA HA) _ nB.
+      apply: IH erefl (expand_det_tree Hz fA HA) _ nB.
   Qed.
 
   Definition is_det A := forall s s' B,
@@ -591,7 +815,7 @@ Section check.
 
   Lemma runb_next_alt {sP A}: 
     check_program sP -> 
-      no_free_alt sP A -> is_det A.
+      det_tree sP A -> is_det A.
   Proof.
     rewrite/is_det.
     move=> H1 H2 s s' B []b H3.
@@ -606,7 +830,7 @@ Section check.
   Qed.
 
   Lemma main {sP p t}:
-    check_program sP -> tm_is_det sP t -> 
+    check_program sP -> callable_is_det sP t -> 
       is_det ((CallS p t)).
   Proof.
     move=> H1 fA HA.
@@ -640,7 +864,7 @@ Section check.
     Qed.
 
     Lemma tail_cut_is_det sP p t:
-      AllTailCut -> tm_is_det sP t -> is_det ((CallS p t)).
+      AllTailCut -> callable_is_det sP t -> is_det ((CallS p t)).
     Proof.
       move=> /(cut_in_prem_tail_cut sP).
       apply main.
